DPA DH

code/ecdsap256/Hacl.Impl.P256.DH.fst
@@ -21,7 +21,23 @@ open Hacl.Impl.P256.Signature.Common
 
 #set-options "--fuel 0 --ifuel 0 --z3rlimit 200"
 
-let ecp256dh_i result scalar =
+inline_for_extraction noextract
+val ecp256dh_i_clear:
+  result:lbuffer uint8 (size 64)
+  -> scalar:lbuffer uint8 (size 32)
+  -> Stack bool
+  (requires fun h ->
+    live h result /\ live h scalar /\ 
+    disjoint result scalar)
+  (ensures fun h0 r h1 ->
+    let pointX, pointY, flag = ecp256_dh_i (as_seq h0 scalar) in
+    modifies (loc result) h0 h1 /\
+    r == flag /\
+    as_seq h1 (gsub result (size 0) (size 32)) == pointX /\
+    as_seq h1 (gsub result (size 32) (size 32)) == pointY)
+
+
+let ecp256dh_i_clear result scalar =
   push_frame();
   let tempBuffer = create (size 100) (u64 0) in
   let resultBuffer = create (size 12) (u64 0) in
@@ -51,6 +67,7 @@ let ecp256dh_i result scalar =
 
   let open Hacl.Impl.P256.LowLevel.RawCmp in 
   unsafe_bool_of_u64  flag
+
 
 
 [@ (Comment "  The pub(lic)_key input of the function is considered to be public, 
@@ -101,7 +118,28 @@ let _ecp256dh_r result pubKey scalar =
     end
 
 
-let ecp256dh_r result pubKey scalar =
+
+
+inline_for_extraction noextract
+val ecp256dh_r_clear:
+    result:lbuffer uint8 (size 64)
+  -> pubKey:lbuffer uint8 (size 64)
+  -> scalar:lbuffer uint8 (size 32)
+  -> Stack bool
+    (requires fun h ->
+      live h result /\ live h pubKey /\ live h scalar /\
+      disjoint result pubKey /\ disjoint result scalar)
+    (ensures fun h0 r h1 ->
+      let pubKeyX = gsub pubKey (size 0) (size 32) in
+      let pubKeyY = gsub pubKey (size 32) (size 32) in
+      let pointX, pointY, flag =
+        ecp256_dh_r (as_seq h0 pubKeyX) (as_seq h0 pubKeyY) (as_seq h0 scalar) in
+      r == flag /\
+      modifies (loc result) h0 h1 /\
+      as_seq h1 (gsub result (size 0) (size 32)) == pointX /\
+      as_seq h1 (gsub result (size 32) (size 32)) == pointY)
+
+let ecp256dh_r_clear  result pubKey scalar =
   push_frame();
   let h0 = ST.get() in
   let resultBufferFelem = create (size 12) (u64 0) in
@@ -149,4 +187,48 @@ let ecp256dh_r result pubKey scalar =
   
   let open Hacl.Impl.P256.LowLevel.RawCmp in 
   unsafe_bool_of_u64  flag
+
+
+
+
+inline_for_extraction noextract
+val ecp256dh_i_bp_hiding:
+  random: felem
+  ->  result:lbuffer uint8 (size 64)
+  -> scalar:lbuffer uint8 (size 32)
+  -> Stack bool
+  (requires fun h ->
+    live h result /\ live h scalar /\ 
+    disjoint result scalar)
+  (ensures fun h0 r h1 ->
+    let pointX, pointY, flag = ecp256_dh_i (as_seq h0 scalar) in
+    modifies (loc result) h0 h1 /\
+    r == flag /\
+    as_seq h1 (gsub result (size 0) (size 32)) == pointX /\
+    as_seq h1 (gsub result (size 32) (size 32)) == pointY)
+
+
+let ecp256dh_i_bp_hiding random result scalar = 
+  let open Hacl.Impl.Q.BasePointBlinding in 
+  push_frame();
+    let tempBuffer = create (size 100) (u64 0) in
+    let basePoint = create (size 12) (u64 0) in 
+    uploadBasePoint basePoint;
+    basePointRandomisation basePoint random;
+    scalarMultiplication basePoint result scalar tempBuffer;
+  pop_frame();
+  true
+  
+
+
+
+let ecp256_dh_i p random result scalar = 
+  match p with 
+  |_ -> ecp256dh_i_clear result scalar
+
+
+
+let ecp256_dh_r p result scalar = 
+  match p with 
+  |_ -> ecp256dh_r_clear p result scalar
 
