code/ecdsap256/Hacl.Impl.P256.DH.fsti
@@ -12,9 +12,17 @@ open Spec.DH
 open Spec.ECDSAP256.Definition
 
 
+type protection = 
+  |BasePointBlinding 
+  |No
+
+
+
 inline_for_extraction noextract
 val ecp256dh_i:
-    result:lbuffer uint8 (size 64)
+  pr: protection
+  -> random: felem
+  -> result:lbuffer uint8 (size 64)
   -> scalar:lbuffer uint8 (size 32)
   -> Stack bool
   (requires fun h ->
